Bring back old proofs

Regex/NFA/Transition.lean
@@ -8,455 +8,387 @@ import Mathlib.Data.Set.Lattice
 open Set
 
 -- TODO: we may want to prove that all indices are in bounds get rid of Option helpers.
--- def Option.charStep : Option NFA.Node → Char → Set Nat
---   | some n, c => n.charStep c
---   | none, _ => ∅
+def Option.charStep : Option NFA.Node → Char → Set Nat
+  | some n, c => n.charStep c
+  | none, _ => ∅
 
--- def Option.εStep : Option NFA.Node → Set Nat
---   | some n => n.εStep
---   | none => ∅
+def Option.εStep : Option NFA.Node → Set Nat
+  | some n => n.εStep
+  | none => ∅
 
 namespace NFA
 
--- def Option.charStep.simp {nfa : NFA} {i : Nat} {c : Char} :
---   nfa[i]?.charStep c = if h : i < nfa.nodes.size then nfa[i].charStep c else ∅ := by
---   simp [Option.charStep, getElem?]
---   cases Nat.decLt i nfa.nodes.size <;> simp [*]
+def Option.charStep.simp {nfa : NFA} {i : Nat} {c : Char} :
+  nfa[i]?.charStep c = if h : i < nfa.nodes.size then nfa[i].charStep c else ∅ := by
+  simp [Option.charStep, getElem?]
+  cases Nat.decLt i nfa.nodes.size <;> simp [*]
 
--- theorem Option.charStep.subset_of_le {nfa₁ nfa₂ : NFA} {i : Nat} (le : nfa₁ ≤ nfa₂) :
---   nfa₁[i]?.charStep c ⊆ nfa₂[i]?.charStep c := by
---   simp [Option.charStep.simp]
---   cases Nat.decLt i nfa₁.nodes.size <;> simp [*]
---   case isTrue h =>
---     let ⟨h', le⟩ := le i h
---     simp [h']
---     exact le.left c
+theorem Option.charStep.subset_of_le {nfa₁ nfa₂ : NFA} {i : Nat} (le : nfa₁ ≤ nfa₂) :
+  nfa₁[i]?.charStep c ⊆ nfa₂[i]?.charStep c := by
+  simp [Option.charStep.simp]
+  cases Nat.decLt i nfa₁.nodes.size <;> simp [*]
+  case isTrue h =>
+    let ⟨h', le⟩ := le i h
+    simp [h']
+    exact le.left c
 
--- def Option.εStep.simp {nfa : NFA} {i : Nat} :
---   nfa[i]?.εStep = if h : i < nfa.nodes.size then nfa[i].εStep else ∅ := by
---   simp [Option.εStep, getElem?]
---   cases Nat.decLt i nfa.nodes.size <;> simp [*]
+def Option.εStep.simp {nfa : NFA} {i : Nat} :
+  nfa[i]?.εStep = if h : i < nfa.nodes.size then nfa[i].εStep else ∅ := by
+  simp [Option.εStep, getElem?]
+  cases Nat.decLt i nfa.nodes.size <;> simp [*]
 
--- theorem Option.εStep.subset_of_le {nfa₁ nfa₂ : NFA} {i : Nat} (le : nfa₁ ≤ nfa₂) :
---   nfa₁[i]?.εStep ⊆ nfa₂[i]?.εStep := by
---   simp [Option.εStep.simp]
---   cases Nat.decLt i nfa₁.nodes.size <;> simp [*]
---   case isTrue h =>
---     let ⟨h', le⟩ := le i h
---     simp [h']
---     exact le.right
+theorem Option.εStep.subset_of_le {nfa₁ nfa₂ : NFA} {i : Nat} (le : nfa₁ ≤ nfa₂) :
+  nfa₁[i]?.εStep ⊆ nfa₂[i]?.εStep := by
+  simp [Option.εStep.simp]
+  cases Nat.decLt i nfa₁.nodes.size <;> simp [*]
+  case isTrue h =>
+    let ⟨h', le⟩ := le i h
+    simp [h']
+    exact le.right
 
--- inductive NFA.εClosure (nfa : NFA) : Nat → Set Nat where
---   | base : εClosure nfa i i
---   | step {i j k : Nat} (head : j ∈ nfa[i]?.εStep) (tail : nfa.εClosure j k) :
---     εClosure nfa i k
+inductive NFA.εClosure (nfa : NFA) : Nat → Set Nat where
+  | base : εClosure nfa i i
+  | step {i j k : Nat} (head : j ∈ nfa[i]?.εStep) (tail : nfa.εClosure j k) :
+    εClosure nfa i k
 
--- theorem εClosure_of_le {nfa₁ nfa₂ : NFA} (le : nfa₁ ≤ nfa₂) (h : j ∈ nfa₁.εClosure i) :
---   j ∈ nfa₂.εClosure i := by
---   induction h with
---   | base => exact .base
---   | step head _ ih => exact .step (mem_of_subset_of_mem (Option.εStep.subset_of_le le) head) ih
+theorem εClosure_of_le {nfa₁ nfa₂ : NFA} (le : nfa₁ ≤ nfa₂) (h : j ∈ nfa₁.εClosure i) :
+  j ∈ nfa₂.εClosure i := by
+  induction h with
+  | base => exact .base
+  | step head _ ih => exact .step (mem_of_subset_of_mem (Option.εStep.subset_of_le le) head) ih
 
--- theorem εClosure_subset_of_le {nfa₁ nfa₂ : NFA} (le : nfa₁ ≤ nfa₂) :
---   nfa₁.εClosure i ⊆ nfa₂.εClosure i := by
---   intro j h
---   exact εClosure_of_le le h
+theorem εClosure_subset_of_le {nfa₁ nfa₂ : NFA} (le : nfa₁ ≤ nfa₂) :
+  nfa₁.εClosure i ⊆ nfa₂.εClosure i := by
+  intro j h
+  exact εClosure_of_le le h
 
--- theorem εClosure_trans {nfa : NFA} (h₁ : i₂ ∈ nfa.εClosure i₁) (h₂ : i₃ ∈ nfa.εClosure i₂) :
---   i₃ ∈ nfa.εClosure i₁ := by
---   induction h₁ with
---   | base => exact h₂
---   | step head _ ih => exact .step head (ih h₂)
+theorem εClosure_trans {nfa : NFA} (h₁ : i₂ ∈ nfa.εClosure i₁) (h₂ : i₃ ∈ nfa.εClosure i₂) :
+  i₃ ∈ nfa.εClosure i₁ := by
+  induction h₁ with
+  | base => exact h₂
+  | step head _ ih => exact .step head (ih h₂)
 
--- def NFA.εClosureSet (nfa : NFA) (S : Set Nat) : Set Nat :=
---   ⋃ i ∈ S, nfa.εClosure i
+def NFA.εClosureSet (nfa : NFA) (S : Set Nat) : Set Nat :=
+  ⋃ i ∈ S, nfa.εClosure i
 
--- @[simp]
--- theorem subset_εClosureSet {nfa : NFA} : S ⊆ nfa.εClosureSet S := by
---   intro i h
---   apply mem_iUnion_of_mem i
---   simp
---   exact ⟨h, .base⟩
+@[simp]
+theorem subset_εClosureSet {nfa : NFA} : S ⊆ nfa.εClosureSet S := by
+  intro i h
+  apply mem_iUnion_of_mem i
+  simp
+  exact ⟨h, .base⟩
 
--- @[simp]
--- theorem εClosureSet_singleton_base {nfa : NFA} : i ∈ nfa.εClosureSet {i} := by
---   apply mem_iUnion_of_mem i
---   simp
---   exact .base
+@[simp]
+theorem εClosureSet_singleton_base {nfa : NFA} : i ∈ nfa.εClosureSet {i} := by
+  apply mem_iUnion_of_mem i
+  simp
+  exact .base
 
--- @[simp]
--- theorem εClosureSet_singleton_step {nfa : NFA} {i j : Nat} (h : j ∈ nfa[i]?.εStep) : j ∈ nfa.εClosureSet {i} := by
---   apply mem_iUnion_of_mem i
---   simp
---   exact .step h .base
+@[simp]
+theorem εClosureSet_singleton_step {nfa : NFA} {i j : Nat} (h : j ∈ nfa[i]?.εStep) : j ∈ nfa.εClosureSet {i} := by
+  apply mem_iUnion_of_mem i
+  simp
+  exact .step h .base
 
--- @[simp]
--- theorem εClosureSet_singleton {nfa : NFA} {i j : Nat} (h : j ∈ nfa.εClosure i):
---   j ∈ nfa.εClosureSet {i} := by
---   apply mem_iUnion_of_mem i
---   simp [h]
+@[simp]
+theorem εClosureSet_singleton {nfa : NFA} {i j : Nat} (h : j ∈ nfa.εClosure i):
+  j ∈ nfa.εClosureSet {i} := by
+  apply mem_iUnion_of_mem i
+  simp [h]
 
--- @[simp]
--- theorem εClosureSet_empty {nfa : NFA} : nfa.εClosureSet ∅ = ∅ := by
---   simp [NFA.εClosureSet]
+@[simp]
+theorem εClosureSet_empty {nfa : NFA} : nfa.εClosureSet ∅ = ∅ := by
+  simp [NFA.εClosureSet]
 
--- @[simp]
--- theorem εClosureSet_univ {nfa : NFA} : nfa.εClosureSet univ = univ :=
---   univ_subset_iff.mp subset_εClosureSet
+@[simp]
+theorem εClosureSet_univ {nfa : NFA} : nfa.εClosureSet univ = univ :=
+  univ_subset_iff.mp subset_εClosureSet
 
--- theorem εClosureSet_subset {nfa₁ nfa₂ : NFA} (hn : nfa₁ ≤ nfa₂) (hs : S₁ ⊆ S₂) :
---   nfa₁.εClosureSet S₁ ⊆ nfa₂.εClosureSet S₂ := by
---   apply biUnion_mono hs
---   intro i _
---   exact εClosure_subset_of_le hn
+theorem εClosureSet_subset {nfa₁ nfa₂ : NFA} (hn : nfa₁ ≤ nfa₂) (hs : S₁ ⊆ S₂) :
+  nfa₁.εClosureSet S₁ ⊆ nfa₂.εClosureSet S₂ := by
+  apply biUnion_mono hs
+  intro i _
+  exact εClosure_subset_of_le hn
 
--- @[simp]
--- theorem εClosureSet_idempotent {nfa : NFA} : nfa.εClosureSet (nfa.εClosureSet S) = nfa.εClosureSet S := by
---   apply eq_of_subset_of_subset
---   . simp [subset_def]
---     intro k h
---     simp [mem_iUnion, NFA.εClosureSet] at h
---     let ⟨i, h, j, cls, cls'⟩ := h
---     exact mem_iUnion_of_mem i (mem_iUnion_of_mem h (εClosure_trans cls cls'))
---   . apply subset_εClosureSet
+@[simp]
+theorem εClosureSet_idempotent {nfa : NFA} : nfa.εClosureSet (nfa.εClosureSet S) = nfa.εClosureSet S := by
+  apply eq_of_subset_of_subset
+  . simp [subset_def]
+    intro k h
+    simp [mem_iUnion, NFA.εClosureSet] at h
+    let ⟨i, h, j, cls, cls'⟩ := h
+    exact mem_iUnion_of_mem i (mem_iUnion_of_mem h (εClosure_trans cls cls'))
+  . apply subset_εClosureSet
 
--- theorem εClosureSet_iUnion_distrib {nfa : NFA} {S : Set α} {f : α → Set Nat} :
---   nfa.εClosureSet (⋃ i ∈ S, f i) = ⋃ i ∈ S, nfa.εClosureSet (f i) := by
---   simp [NFA.εClosureSet]
+theorem εClosureSet_iUnion_distrib {nfa : NFA} {S : Set α} {f : α → Set Nat} :
+  nfa.εClosureSet (⋃ i ∈ S, f i) = ⋃ i ∈ S, nfa.εClosureSet (f i) := by
+  simp [NFA.εClosureSet]
 
--- theorem εClosureSet_union_distrib {nfa : NFA} {S₁ S₂ : Set Nat} :
---   nfa.εClosureSet (S₁ ∪ S₂) = nfa.εClosureSet S₁ ∪ nfa.εClosureSet S₂ := by
---   apply eq_of_subset_of_subset
---   . simp [subset_def]
---     intro j h
---     simp [NFA.εClosureSet] at *
---     let ⟨i, h, cls⟩ := h
---     cases h with
---     | inl h => exact .inl ⟨i, h, cls⟩
---     | inr h => exact .inr ⟨i, h, cls⟩
---   . simp [subset_def]
---     intro j h
---     simp [NFA.εClosureSet] at *
---     cases h with
---     | inl h =>
---       let ⟨i, h, cls⟩ := h
---       exact ⟨i, .inl h, cls⟩
---     | inr h =>
---       let ⟨i, h, cls⟩ := h
---       exact ⟨i, .inr h, cls⟩
+theorem εClosureSet_union_distrib {nfa : NFA} {S₁ S₂ : Set Nat} :
+  nfa.εClosureSet (S₁ ∪ S₂) = nfa.εClosureSet S₁ ∪ nfa.εClosureSet S₂ := by
+  apply eq_of_subset_of_subset
+  . simp [subset_def]
+    intro j h
+    simp [NFA.εClosureSet] at *
+    let ⟨i, h, cls⟩ := h
+    cases h with
+    | inl h => exact .inl ⟨i, h, cls⟩
+    | inr h => exact .inr ⟨i, h, cls⟩
+  . simp [subset_def]
+    intro j h
+    simp [NFA.εClosureSet] at *
+    cases h with
+    | inl h =>
+      let ⟨i, h, cls⟩ := h
+      exact ⟨i, .inl h, cls⟩
+    | inr h =>
+      let ⟨i, h, cls⟩ := h
+      exact ⟨i, .inr h, cls⟩
 
--- def NFA.stepSet (nfa : NFA) (S : Set Nat) (c : Char) : Set Nat :=
---   ⋃ i ∈ S, nfa.εClosureSet (nfa[i]?.charStep c)
+def NFA.stepSet (nfa : NFA) (S : Set Nat) (c : Char) : Set Nat :=
+  ⋃ i ∈ S, nfa.εClosureSet (nfa[i]?.charStep c)
 
--- @[simp]
--- def stepSet_empty {nfa : NFA} : nfa.stepSet ∅ c = ∅ := by
---   simp [NFA.stepSet]
+@[simp]
+def stepSet_empty {nfa : NFA} : nfa.stepSet ∅ c = ∅ := by
+  simp [NFA.stepSet]
 
--- @[simp]
--- theorem εClosureSet_stepSet {nfa : NFA} :
---   nfa.εClosureSet (nfa.stepSet S c) = nfa.stepSet S c := by
---   apply eq_of_subset_of_subset
---   . conv =>
---       lhs
---       simp [NFA.stepSet, εClosureSet_iUnion_distrib]
---   . exact subset_εClosureSet
+@[simp]
+theorem εClosureSet_stepSet {nfa : NFA} :
+  nfa.εClosureSet (nfa.stepSet S c) = nfa.stepSet S c := by
+  apply eq_of_subset_of_subset
+  . conv =>
+      lhs
+      simp [NFA.stepSet, εClosureSet_iUnion_distrib]
+  . exact subset_εClosureSet
 
--- theorem stepSet_subset {nfa₁ nfa₂ : NFA} (hn : nfa₁ ≤ nfa₂) (hs : S₁ ⊆ S₂) :
---   nfa₁.stepSet S₁ c ⊆ nfa₂.stepSet S₂ c := by
---   simp [subset_def, NFA.stepSet]
---   intro j i h₁ h₂
+theorem stepSet_subset {nfa₁ nfa₂ : NFA} (hn : nfa₁ ≤ nfa₂) (hs : S₁ ⊆ S₂) :
+  nfa₁.stepSet S₁ c ⊆ nfa₂.stepSet S₂ c := by
+  simp [subset_def, NFA.stepSet]
+  intro j i h₁ h₂
 
---   exact ⟨
---     i,
---     mem_of_subset_of_mem hs h₁,
---     mem_of_subset_of_mem (εClosureSet_subset hn (Option.charStep.subset_of_le hn)) h₂
---   ⟩
+  exact ⟨
+    i,
+    mem_of_subset_of_mem hs h₁,
+    mem_of_subset_of_mem (εClosureSet_subset hn (Option.charStep.subset_of_le hn)) h₂
+  ⟩
 
--- def NFA.evalFrom (nfa : NFA) (S : Set Nat) : List Char → Set Nat :=
---   List.foldl (nfa.stepSet) (nfa.εClosureSet S)
+def NFA.evalFrom (nfa : NFA) (S : Set Nat) : List Char → Set Nat :=
+  List.foldl (nfa.stepSet) (nfa.εClosureSet S)
 
--- theorem evalFrom_cons {nfa : NFA} :
---   nfa.evalFrom S (c :: cs) = nfa.evalFrom (nfa.stepSet (nfa.εClosureSet S) c) cs := by
---   have h : nfa.stepSet (nfa.εClosureSet S) c = nfa.εClosureSet (nfa.stepSet (nfa.εClosureSet S) c) :=
---     εClosureSet_stepSet.symm
---   conv =>
---     lhs
---     simp [NFA.evalFrom]
---     rw [h]
+theorem evalFrom_cons {nfa : NFA} :
+  nfa.evalFrom S (c :: cs) = nfa.evalFrom (nfa.stepSet (nfa.εClosureSet S) c) cs := by
+  have h : nfa.stepSet (nfa.εClosureSet S) c = nfa.εClosureSet (nfa.stepSet (nfa.εClosureSet S) c) :=
+    εClosureSet_stepSet.symm
+  conv =>
+    lhs
+    simp [NFA.evalFrom]
+    rw [h]
 
--- theorem evalFrom_subset {nfa₁ nfa₂ : NFA} {S₁ S₂ : Set Nat} (hn : nfa₁ ≤ nfa₂) (hs : S₁ ⊆ S₂) :
---   nfa₁.evalFrom S₁ s ⊆ nfa₂.evalFrom S₂ s := by
---   apply le_foldl_of_le
---   . intro _ _ _ hs
---     exact stepSet_subset hn hs
---   . exact εClosureSet_subset hn hs
+theorem evalFrom_subset {nfa₁ nfa₂ : NFA} {S₁ S₂ : Set Nat} (hn : nfa₁ ≤ nfa₂) (hs : S₁ ⊆ S₂) :
+  nfa₁.evalFrom S₁ s ⊆ nfa₂.evalFrom S₂ s := by
+  apply le_foldl_of_le
+  . intro _ _ _ hs
+    exact stepSet_subset hn hs
+  . exact εClosureSet_subset hn hs
 
--- theorem εClosureSet_evalFrom {nfa : NFA} :
---   nfa.εClosureSet (nfa.evalFrom S s) = nfa.evalFrom S s := by
---   apply eq_of_subset_of_subset
---   . induction s generalizing S with
---     | nil => simp [NFA.evalFrom]; exact le_refl _
---     | cons c cs ih =>
---       rw [evalFrom_cons]
---       exact ih
---   . exact subset_εClosureSet
+theorem εClosureSet_evalFrom {nfa : NFA} :
+  nfa.εClosureSet (nfa.evalFrom S s) = nfa.evalFrom S s := by
+  apply eq_of_subset_of_subset
+  . induction s generalizing S with
+    | nil => simp [NFA.evalFrom]; exact le_refl _
+    | cons c cs ih =>
+      rw [evalFrom_cons]
+      exact ih
+  . exact subset_εClosureSet
 
--- theorem mem_evalFrom_subset {nfa : NFA} (hmem : next ∈ nfa.evalFrom S₁ s) (hs : S₁ ⊆ nfa.εClosureSet S₂) :
---   next ∈ nfa.evalFrom S₂ s := by
---   apply mem_of_subset_of_mem _ hmem
---   apply le_foldl_of_le
---   . intro _ _ _ hs
---     exact stepSet_subset (le_refl _) hs
---   . suffices nfa.εClosureSet S₁ ⊆ nfa.εClosureSet (nfa.εClosureSet S₂) by
---       simp at this
---       exact this
---     exact εClosureSet_subset (le_refl _) hs
+theorem mem_evalFrom_subset {nfa : NFA} (hmem : next ∈ nfa.evalFrom S₁ s) (hs : S₁ ⊆ nfa.εClosureSet S₂) :
+  next ∈ nfa.evalFrom S₂ s := by
+  apply mem_of_subset_of_mem _ hmem
+  apply le_foldl_of_le
+  . intro _ _ _ hs
+    exact stepSet_subset (le_refl _) hs
+  . suffices nfa.εClosureSet S₁ ⊆ nfa.εClosureSet (nfa.εClosureSet S₂) by
+      simp at this
+      exact this
+    exact εClosureSet_subset (le_refl _) hs
 
--- theorem evalFrom_append {nfa : NFA} (eq : s = s₁ ++ s₂) :
---   nfa.evalFrom S s = List.foldl (nfa.stepSet) (nfa.evalFrom S s₁) s₂ := by
---   conv =>
---     lhs
---     rw [eq, NFA.evalFrom, List.foldl_append]
+theorem evalFrom_append {nfa : NFA} (eq : s = s₁ ++ s₂) :
+  nfa.evalFrom S s = List.foldl (nfa.stepSet) (nfa.evalFrom S s₁) s₂ := by
+  conv =>
+    lhs
+    rw [eq, NFA.evalFrom, List.foldl_append]
 
--- theorem mem_evalFrom_le {nfa₁ nfa₂ : NFA} (le : nfa₁ ≤ nfa₂) (h : next ∈ nfa₁.evalFrom S s) :
---   next ∈ nfa₂.evalFrom S s :=
---   evalFrom_subset le (le_refl _) h
+theorem mem_evalFrom_le {nfa₁ nfa₂ : NFA} (le : nfa₁ ≤ nfa₂) (h : next ∈ nfa₁.evalFrom S s) :
+  next ∈ nfa₂.evalFrom S s :=
+  evalFrom_subset le (le_refl _) h
 
--- open NFA
+theorem evalFrom_of_matches (eq : compile.loop r next nfa = nfa')
+  (m : r.matches s) : ∀ nfa'' : NFA, nfa' ≤ nfa'' → next ∈ nfa''.evalFrom {nfa'.val.start.val} s.data := by
+  induction m generalizing next nfa with
+  | @char s c eqs =>
+    intro nfa'' le
+    apply mem_evalFrom_le le
+    simp [eqs, NFA.evalFrom, List.foldl]
+    simp [compile.loop] at eq
+    apply mem_iUnion_of_mem nfa'.val.start.val
+    subst eq
+    simp [Option.charStep, Node.charStep]
+  | @epsilon s eqs =>
+    intro nfa'' le
+    apply mem_evalFrom_le le
+    simp [eqs, NFA.evalFrom, List.foldl]
+    simp [compile.loop] at eq
+    apply mem_iUnion_of_mem nfa'.val.start.val
+    subst eq
+    simp [Option.charStep, Node.charStep]
+    exact NFA.εClosure.step (by simp [Option.εStep, Node.εStep]) .base
+  | @alternateLeft s r₁ r₂ _ ih =>
+    intro nfa'' le
+    apply mem_evalFrom_le le
 
--- theorem evalFrom_of_matches (eq : compile.loop r next nfa = nfa')
---   (m : r.matches s) : ∀ nfa'' : NFA, nfa' ≤ nfa'' → next ∈ nfa''.evalFrom {nfa'.val.start.val} s.data := by
---   induction m generalizing next nfa with
---   | @char s c eqs =>
---     intro nfa'' le
---     apply mem_evalFrom_le le
---     simp [eqs, evalFrom, List.foldl]
---     simp [compile.loop] at eq
---     apply mem_iUnion_of_mem nfa'.val.start.val
---     subst eq
---     simp [Option.charStep, Node.charStep]
---   | @epsilon s eqs =>
---     intro nfa'' le
---     apply mem_evalFrom_le le
---     simp [eqs, evalFrom, List.foldl]
---     simp [compile.loop] at eq
---     apply mem_iUnion_of_mem nfa'.val.start.val
---     subst eq
---     simp [Option.charStep, Node.charStep]
---     exact εClosure.step (by simp [Option.εStep, Node.εStep]) .base
---   | @alternateLeft s r₁ r₂ _ ih =>
---     intro nfa'' le
---     apply mem_evalFrom_le le
+    apply compile.loop.alternate eq
+    intro nfa₁ start₁ nfa₂ start₂ final property eq₁ eq₂ _ _ eq₅ eq
 
---     apply compile.loop.alternate eq
---     intro nfa₁ start₁ nfa₂ start₂ final property eq₁ eq₂ _ _ eq₅ eq
+    have property : nfa₁.val ≤ final.val :=
+      calc nfa₁.val
+        _ ≤ nfa₂.val := nfa₂.property
+        _ ≤ final.val := final.property
 
---     have property : nfa₁.val ≤ final.val :=
---       calc nfa₁.val
---         _ ≤ nfa₂.val := nfa₂.property
---         _ ≤ final.val := final.property
+    rw [eq]
+    simp
 
---     rw [eq]
---     simp
+    apply mem_evalFrom_subset (ih eq₁.symm final property)
+    simp
+    apply εClosureSet_singleton_step
+    rw [eq₅]
+    simp [Option.εStep, Node.εStep]
+    exact .inl (by rw [eq₂])
+  | @alternateRight s r₁ r₂ _ ih =>
+    intro nfa'' le
+    apply mem_evalFrom_le le
 
---     apply mem_evalFrom_subset (ih eq₁.symm final property)
---     simp
---     apply εClosureSet_singleton_step
---     rw [eq₅]
---     simp [Option.εStep, Node.εStep]
---     exact .inl (by rw [eq₂])
---   | @alternateRight s r₁ r₂ _ ih =>
---     intro nfa'' le
---     apply mem_evalFrom_le le
+    apply compile.loop.alternate eq
+    intro nfa₁ start₁ nfa₂ start₂ final property _ _ eq₃ eq₄ eq₅ eq
 
---     apply compile.loop.alternate eq
---     intro nfa₁ start₁ nfa₂ start₂ final property _ _ eq₃ eq₄ eq₅ eq
+    rw [eq]
+    simp
 
---     rw [eq]
---     simp
+    apply mem_evalFrom_subset (ih eq₃.symm final final.property)
+    simp
+    apply εClosureSet_singleton_step
+    rw [eq₅]
+    simp [Option.εStep, Node.εStep]
+    exact .inr (by rw [eq₄])
+  | concat s s₁ s₂ r₁ r₂ eqs _ _ ih₁ ih₂ =>
+    intro nfa'' le
+    apply mem_evalFrom_le le
 
---     apply mem_evalFrom_subset (ih eq₃.symm final final.property)
---     simp
---     apply εClosureSet_singleton_step
---     rw [eq₅]
---     simp [Option.εStep, Node.εStep]
---     exact .inr (by rw [eq₄])
---   | concat s s₁ s₂ r₁ r₂ eqs _ _ ih₁ ih₂ =>
---     intro nfa'' le
---     apply mem_evalFrom_le le
+    apply compile.loop.concat eq
+    intro nfa₂ nfa₁ property eq₂ eq₁ eq
 
---     apply compile.loop.concat eq
---     intro nfa₂ nfa₁ property eq₂ eq₁ eq
+    rw [eq]
+    simp
 
---     rw [eq]
---     simp
+    let ih₁ := ih₁ eq₁.symm nfa₁ (le_refl _)
+    let ih₂ := ih₂ eq₂.symm nfa₁ nfa₁.property
 
---     let ih₁ := ih₁ eq₁.symm nfa₁ (le_refl _)
---     let ih₂ := ih₂ eq₂.symm nfa₁ nfa₁.property
+    apply mem_of_mem_of_subset ih₂
+    rw [evalFrom_append (String.eq_of_append_of_eq_of_append eqs)]
+    apply le_foldl_of_le
+    . intro _ _ _ hs
+      exact stepSet_subset (le_refl _) hs
+    . have : {nfa₂.val.start.val} ⊆ nfa₁.val.evalFrom {nfa₁.val.start.val} s₁.data := by
+        rw [singleton_subset_iff]
+        exact ih₁
+      have : nfa₁.val.εClosureSet {nfa₂.val.start.val} ⊆ nfa₁.val.εClosureSet (nfa₁.val.evalFrom {nfa₁.val.start.val} s₁.data) :=
+        εClosureSet_subset (le_refl _) this
+      rw [εClosureSet_evalFrom] at this
+      exact this
+  | starEpsilon eqs =>
+    intro nfa'' le
+    apply mem_evalFrom_le le
 
---     apply mem_of_mem_of_subset ih₂
---     rw [evalFrom_append (String.eq_of_append_of_eq_of_append eqs)]
---     apply le_foldl_of_le
---     . intro _ _ _ hs
---       exact stepSet_subset (le_refl _) hs
---     . have : {nfa₂.val.start.val} ⊆ nfa₁.val.evalFrom {nfa₁.val.start.val} s₁.data := by
---         rw [singleton_subset_iff]
---         exact ih₁
---       have : nfa₁.val.εClosureSet {nfa₂.val.start.val} ⊆ nfa₁.val.εClosureSet (nfa₁.val.evalFrom {nfa₁.val.start.val} s₁.data) :=
---         εClosureSet_subset (le_refl _) this
---       rw [εClosureSet_evalFrom] at this
---       exact this
---   | starEpsilon eqs =>
---     intro nfa'' le
---     apply mem_evalFrom_le le
+    apply compile.loop.star eq
+    intro nfa' start nfa'' nodes''' nfa''' isLt isLt' property'
+      _ _ _ eq₄ eq₅ eq'
 
---     apply compile.loop.star eq
---     intro nfa' start nfa'' nodes''' nfa''' isLt isLt' property'
---       _ _ _ eq₄ eq₅ eq'
+    rw [eq']
+    simp
 
---     rw [eq']
---     simp
+    simp [eqs, NFA.evalFrom, NFA.εClosureSet]
 
---     simp [eqs, NFA.evalFrom, NFA.εClosureSet]
+    have : nfa'''[nfa'''.start.val] = .split nfa''.val.start next := by
+      rw [eq₅, NFA.eq_get]
+      simp [eq₄]
+    have head : next ∈ nfa'''[nfa'''.start]?.εStep := by
+      unfold getElem?
+      simp [this, Option.εStep, Node.εStep]
+    have tail : next ∈ nfa'''.εClosure next := .base
+    exact NFA.εClosure.step head tail
+  | starConcat s s₁ s₂ r eqs _ _ ih₁ ih₂ =>
+    intro nfa'' le
+    apply mem_evalFrom_le le
 
---     have : nfa'''[nfa'''.start.val] = .split nfa''.val.start next := by
---       rw [eq₅, NFA.eq_get]
---       simp [eq₄]
---     have head : next ∈ nfa'''[nfa'''.start]?.εStep := by
---       unfold getElem?
---       simp [this, Option.εStep, Node.εStep]
---     have tail : next ∈ nfa'''.εClosure next := .base
---     exact NFA.εClosure.step head tail
---   | starConcat s s₁ s₂ r eqs _ _ ih₁ ih₂ =>
---     intro nfa'' le
---     apply mem_evalFrom_le le
+    apply compile.loop.star eq
+    intro nfa' start nfa'' nodes''' nfa''' isLt isLt' property'
+      eq₁ eq₂ eq₃ eq₄ eq₅ eq'
 
---     apply compile.loop.star eq
---     intro nfa' start nfa'' nodes''' nfa''' isLt isLt' property'
---       eq₁ eq₂ eq₃ eq₄ eq₅ eq'
+    rw [eq']
+    simp
 
---     rw [eq']
---     simp
+    have eq'' : compile.loop (.star r) next nfa = ⟨nfa''', property'⟩ := by
+      rw [eq'] at eq
+      exact eq
+    have : nfa''.val ≤ nfa''' := by
+      intro i h
+      have : nodes'''.size = nfa''.val.nodes.size := by
+        simp [eq₄]
+      have : i < nodes'''.size := by
+        simp [this, h]
+      have h' : i < nfa'''.nodes.size := by
+        simp [eq₅, this]
+      exists h'
+      cases Nat.decEq start i with
+      | isTrue eq =>
+        have lhs : nfa''.val[i] = .fail := by
+          simp [eq₃, eq.symm]
+          have : start.val < nfa'.val.nodes.size := by
+            rw [eq₂, eq₁]
+            simp
+          simp [compile.loop.get_lt rfl this]
+          have : start.val = (nfa.addNode .fail).val.start.val := by
+            rw [eq₂, eq₁]
+          simp [this, eq₁]
+        have rhs : nfa'''[i] = .split nfa''.val.start next := by
+          simp [NFA.eq_get, eq₅, eq₄, eq.symm]
+        simp [lhs, rhs]
+      | isFalse neq =>
+        have : nodes'''[i] = nfa''.val.nodes[i] := by
+          simp [eq₄]
+          apply Array.get_set_ne
+          exact neq
+        simp [NFA.eq_get, eq₅, this]
+    have ih₁ := ih₁ eq₃.symm nfa''' this
+    have ih₂ := ih₂ eq'' nfa''' (le_refl _)
 
---     have eq'' : compile.loop (.star r) next nfa = ⟨nfa''', property'⟩ := by
---       rw [eq'] at eq
---       exact eq
---     have : nfa''.val ≤ nfa''' := by
---       intro i h
---       have : nodes'''.size = nfa''.val.nodes.size := by
---         simp [eq₄]
---       have : i < nodes'''.size := by
---         simp [this, h]
---       have h' : i < nfa'''.nodes.size := by
---         simp [eq₅, this]
---       exists h'
---       cases Nat.decEq start i with
---       | isTrue eq =>
---         have lhs : nfa''.val[i] = .fail := by
---           simp [eq₃, eq.symm]
---           have : start.val < nfa'.val.nodes.size := by
---             rw [eq₂, eq₁]
---             simp
---           simp [compile.loop.get_lt rfl this]
---           have : start.val = (nfa.addNode .fail).val.start.val := by
---             rw [eq₂, eq₁]
---           simp [this, eq₁]
---         have rhs : nfa'''[i] = .split nfa''.val.start next := by
---           simp [NFA.eq_get, eq₅, eq₄, eq.symm]
---         simp [lhs, rhs]
---       | isFalse neq =>
---         have : nodes'''[i] = nfa''.val.nodes[i] := by
---           simp [eq₄]
---           apply Array.get_set_ne
---           exact neq
---         simp [NFA.eq_get, eq₅, this]
---     have ih₁ := ih₁ eq₃.symm nfa''' this
---     have ih₂ := ih₂ eq'' nfa''' (le_refl _)
+    rw [evalFrom_append (String.eq_of_append_of_eq_of_append eqs)]
+    suffices next ∈ nfa'''.evalFrom (nfa'''.evalFrom {nfa'''.start.val} s₁.data) s₂.data by
+      have : next ∈ List.foldl nfa'''.stepSet (nfa'''.εClosureSet (nfa'''.evalFrom {nfa'''.start.val} s₁.data)) s₂.data := by
+        exact this
+      simp [εClosureSet_evalFrom] at this
+      exact this
+    apply mem_evalFrom_subset ih₂
+    simp [εClosureSet_evalFrom]
 
---     rw [evalFrom_append (String.eq_of_append_of_eq_of_append eqs)]
---     suffices next ∈ nfa'''.evalFrom (nfa'''.evalFrom {nfa'''.start.val} s₁.data) s₂.data by
---       have : next ∈ List.foldl nfa'''.stepSet (nfa'''.εClosureSet (nfa'''.evalFrom {nfa'''.start.val} s₁.data)) s₂.data := by
---         exact this
---       simp [εClosureSet_evalFrom] at this
---       exact this
---     apply mem_evalFrom_subset ih₂
---     simp [εClosureSet_evalFrom]
-
---     have : nfa'''.start.val = start.val := by
---       rw [eq₅]
---     apply mem_evalFrom_subset (this.symm ▸ ih₁)
---     simp
---     apply εClosureSet_singleton_step
---     have : nfa'''[nfa'''.start.val] = .split nfa''.val.start next := by
---       rw [eq₅, NFA.eq_get]
---       simp [eq₄]
---     simp [this, getElem?, Option.εStep, Node.εStep]
-
--- -- こんな感じのが必要では
--- -- def NFA.evalFromUntil (nfa : NFA) (S : Set Nat) (next : Nat) (s : List Char) : Option (List Char) :=
--- --   if next ∈ S then
--- --     some s
--- --   else
--- --     match s with
--- --     | [] => none
--- --     | c :: s => nfa.evalFromUntil (nfa.stepSet S c) next s
-
--- def NFA.stepSet' (nfa : NFA) (S : Set Nat) (c : Char) : Set Nat :=
---   ⋃ i ∈ nfa.εClosureSet S, nfa.εClosureSet (nfa[i]?.charStep c)
-
--- theorem compile.loop.εClosure_subset (eq : compile.loop r next nfa = result)
---   (h : i ∈ NewNodesRange eq) (cls : j ∈ result.val.εClosure i) :
---   j ∈ result.val.εClosure next ∪ NewNodesRange eq := by
---   induction cls with
---   | base => exact Or.inr h
---   | @step i j k head tail ih =>
---     simp [Option.εStep.simp, h.right] at head
---     -- Use whatever char
---     let ⟨_, h⟩ := step_range (c := default) eq i h.left h.right
---     have : j = next ∨ j ∈ NewNodesRange eq := mem_insert_iff.mp (mem_of_mem_of_subset head h)
---     cases this with
---     | inl h => exact mem_union_left _ (h ▸ tail)
---     | inr h => exact ih h
-
--- theorem compile.loop.εClosureSet_NewNodesRange (eq : compile.loop r next nfa = result) :
---   result.val.εClosureSet (NewNodesRange eq) ⊆ result.val.εClosure next ∪ NewNodesRange eq := by
---   simp [NFA.εClosureSet]
---   intro i h
---   simp [subset_def]
---   intro j cls
---   exact εClosure_subset eq h cls
-
--- theorem compile.loop.εClosureSet_subset (eq : compile.loop r next nfa = result)
---   (h : S ⊆ {next} ∪ NewNodesRange eq) :
---   result.val.εClosureSet S ⊆ result.val.εClosure next ∪ NewNodesRange eq := by
---   calc result.val.εClosureSet S
---     _ ⊆ result.val.εClosureSet ({next} ∪ NewNodesRange eq) := by
---       apply NFA.εClosureSet_subset
---       . exact le_refl _
---       . exact h
---     _ = result.val.εClosureSet {next} ∪ result.val.εClosureSet (NewNodesRange eq) :=
---       εClosureSet_union_distrib
---     _ ⊆ result.val.εClosure next ∪ NewNodesRange eq := by
---       simp [εClosureSet_NewNodesRange]
---       simp [εClosureSet]
-
--- theorem compile.loop.stepSet_subset (eq : compile.loop r next nfa = result)
---   (h : S ⊆ NewNodesRange eq) :
---   result.val.stepSet S c ⊆ result.val.εClosure next ∪ NewNodesRange eq := by
---   simp [NFA.stepSet]
---   intro i h'
---   have : i ∈ NewNodesRange eq := mem_of_subset_of_mem h h'
---   have h'' : nfa.nodes.size ≤ i ∧ i < result.val.nodes.size := by
---     simp [NewNodesRange] at this
---     exact this
---   apply εClosureSet_subset eq
---   simp [Option.charStep.simp, h''.right]
---   let ⟨h, _⟩ := step_range c eq i h''.left h''.right
---   exact h
-
--- inductive NFA.eval (nfa : NFA) : Set Nat → List Char → Set Nat → List Char → Prop where
---   | base : nfa.eval S cs S cs
---   | step (rest : nfa.eval (nfa.stepSet' S c) cs S' cs') : nfa.eval S (c :: cs) S' cs'
+    have : nfa'''.start.val = start.val := by
+      rw [eq₅]
+    apply mem_evalFrom_subset (this.symm ▸ ih₁)
+    simp
+    apply εClosureSet_singleton_step
+    have : nfa'''[nfa'''.start.val] = .split nfa''.val.start next := by
+      rw [eq₅, NFA.eq_get]
+      simp [eq₄]
+    simp [this, getElem?, Option.εStep, Node.εStep]
 
 -- Maybe we should recurse from the last as we reason about the last step often
 inductive NFA.pathIn (nfa : NFA) (start : Nat) : Nat → List Char → Nat → List Char → Prop where
